src/Init/Control.lean
@@ -19,4 +19,3 @@ public import Init.Control.ExceptCps
 public import Init.Control.MonadAttach
 public import Init.Control.EState
 public import Init.Control.Do
-public import Init.Control.Ensures
